proof: fix many things in isa

cogent/isa/StringMap.thy
@@ -9,11 +9,27 @@
  *)
 
 theory StringMap
+  imports CParser.StaticFun
+begin 
 
-(* assumes CParser or AutoCorres to find StaticFun *)
-imports StaticFun
+datatype LexOrdChar = LexOrdChar char
 
-begin
+instantiation LexOrdChar :: linorder begin
+
+definition less_eq_LexOrdChar :: "LexOrdChar \<Rightarrow> LexOrdChar \<Rightarrow> bool" where
+  "c \<le> c' \<equiv> case c of LexOrdChar c \<Rightarrow> case c' of LexOrdChar c' \<Rightarrow> (of_char c :: nat) \<le> of_char c'"
+
+definition less_LexOrdChar :: "LexOrdChar \<Rightarrow> LexOrdChar \<Rightarrow> bool" where
+  "(c < c') \<equiv> case c of LexOrdChar c \<Rightarrow> case c' of LexOrdChar c' \<Rightarrow> (of_char c :: nat) < of_char c'"
+
+instance
+  by (standard; force simp add: less_LexOrdChar_def less_eq_LexOrdChar_def less_le_not_le split: LexOrdChar.splits)
+end
+
+lemma LexOrdChar_inj: "inj LexOrdChar"
+  by (meson LexOrdChar.inject injI)
+
+lemmas LexOrdChar_map_eq_iff = inj_map_eq_map[OF LexOrdChar_inj]
 
 datatype LexOrdString = LexOrdString "string"
 
@@ -21,38 +37,21 @@ instantiation LexOrdString :: linorder begin
 
 definition
   less_LexOrdString_def[simp]:
-  "(s < t) = (case s of LexOrdString s' \<Rightarrow> case t of LexOrdString t' \<Rightarrow>
-    (s', t') \<in> lexord {(c, c'). nat_of_char c < nat_of_char c'})"
+  "(s < t) = (case s of LexOrdString s \<Rightarrow> case t of LexOrdString t \<Rightarrow>
+    ord_class.lexordp (map LexOrdChar s) (map LexOrdChar t))"
 
 definition
-  le_LexOrdString_def[simp]:
-  "(s \<le> t) = ((s :: LexOrdString) < t \<or> s = t)"
-
-lemma nat_of_char_trans:
-  "transP (\<lambda>c c'. nat_of_char c < nat_of_char c')"
-  by (auto intro!: transI)
+  less_eq_LexOrdString_def[simp]:
+  "(s \<le> t) = (case s of LexOrdString s \<Rightarrow> case t of LexOrdString t \<Rightarrow>
+    ord_class.lexordp_eq (map LexOrdChar s) (map LexOrdChar t))"
 
 instance
-  apply intro_classes
-      apply (clarsimp split: LexOrdString.split)
-      apply safe[1]
-       apply (drule(1) lexord_trans[OF _ _ nat_of_char_trans])
-       apply (simp add: lexord_irreflexive)
-      apply (simp add: lexord_irreflexive)
-     apply (clarsimp)
-    apply (clarsimp split: LexOrdString.split_asm)
-    apply safe[1]
-    apply (erule(1) lexord_trans)
-    apply (rule nat_of_char_trans)
-   apply (clarsimp split: LexOrdString.split_asm)
-   apply safe[1]
-   apply (drule(1) lexord_trans[OF _ _ nat_of_char_trans])
-   apply (simp add: lexord_irreflexive)
-  apply (clarsimp split: LexOrdString.split)
-  apply (cut_tac x=list and y=lista in lexord_linear)
-   defer
-   apply blast
-  apply (auto simp: nat_of_char_eq_iff)
+  apply standard
+      apply (clarsimp simp add: lexordp_conv_lexordp_eq split: LexOrdString.splits)
+     apply (clarsimp simp add: lexordp_eq_refl split: LexOrdString.splits)
+    apply (force dest: lexordp_eq_trans split: LexOrdString.splits)
+   apply (auto dest!: lexordp_eq_antisym simp add: LexOrdChar_map_eq_iff lexordp_eq_refl split: LexOrdString.splits)[1]
+  apply (clarsimp simp add: lexordp_eq_linear split: LexOrdString.splits)
   done
 
 end
@@ -65,7 +64,7 @@ fun define_string_map name assocs ctxt = let
     val th_names = map (prefix (Binding.name_of name ^ "_") o fst) assocs
     val mappings = map (apfst HOLogic.mk_string) assocs
   in StaticFun.define_tree_and_save_thms name th_names mappings
-    @{term LexOrdString} @{thms nat_of_char_def} ctxt end
+    @{term LexOrdString} @{thms of_char_def less_eq_LexOrdChar_def less_LexOrdChar_def} ctxt end
 
 end
 
