cogent/isa/TypeTrackingSemantics.thy
@@ -32,8 +32,8 @@ fun
   follow_typing_tree :: "tree_ctx \<Rightarrow> tree_ctx \<times> tree_ctx"
 where
   "follow_typing_tree (TyTrSplit sps xs T1 ys T2, \<Gamma>)
-    = ((T1, xs @ map (fst o Product_Type.split apply_tsk) (zip sps \<Gamma>)),
-        (T2, ys @ map (snd o Product_Type.split apply_tsk) (zip sps \<Gamma>)))"
+    = ((T1, xs @ map (fst o case_prod apply_tsk) (zip sps \<Gamma>)),
+        (T2, ys @ map (snd o case_prod apply_tsk) (zip sps \<Gamma>)))"
 
 fun
   new_tt_types :: "tree_ctx \<Rightarrow> ctx"
@@ -206,35 +206,37 @@ lemma split_bang_nth:
    apply (auto elim: split_bang.cases intro: split_bang_empty)[1]
   apply (rule iffI)
    apply (erule split_bang.cases, simp)
-    apply (clarsimp split del: split_if)
+    apply clarsimp
     apply (case_tac i)
      apply simp
-    apply (simp add: Suc_mem_image_pred split del: split_if cong: if_cong)
-   apply (clarsimp split del: split_if)
+    apply (simp add: Suc_mem_image_pred cong: if_cong)
+   apply clarsimp
    apply (case_tac i)
     apply simp
-   apply (simp add: Suc_mem_image_pred_remove split del: split_if cong: if_cong)
+   apply (simp add: Suc_mem_image_pred_remove cong: if_cong)
   apply (clarsimp simp: length_Suc_conv forall_less_Suc_eq)
   apply (frule_tac x=0 in spec, simp(no_asm_use))
   apply (case_tac "0 \<in> is", simp_all)
    apply clarsimp
    apply (erule split_bang_bang, rule refl)
-   apply (simp add: Suc_mem_image_pred_remove split del: split_if cong: if_cong)
-  apply (rule split_bang_cons, (simp_all add: Suc_mem_image_pred split del: split_if cong: if_cong))
+   apply (simp add: Suc_mem_image_pred_remove cong: if_cong)
+  apply (rule split_bang_cons, (simp_all add: Suc_mem_image_pred cong: if_cong))
   done
 
 lemma ttsplit_bang_imp_split_bang:
   "ttsplit_bang is sps K \<Gamma> xs \<Gamma>1 ys \<Gamma>2 \<Longrightarrow>
     (\<exists>\<Gamma>1a \<Gamma>2a. split_bang K is (snd \<Gamma>) \<Gamma>1a \<Gamma>2a
         \<and> snd \<Gamma>1 = xs @ \<Gamma>1a & snd \<Gamma>2 = ys @ \<Gamma>2a)"
-  apply (clarsimp simp: ttsplit_bang_def ttsplit_bang_inner_def
-                        split_bang_nth nth_enumerate_eq
-              split del: split_if cong: if_cong)
+  apply (clarsimp
+      simp: ttsplit_bang_def ttsplit_bang_inner_def split_bang_nth nth_enumerate_eq
+      cong: if_cong)
+  apply (case_tac "sps ! i")
+   apply (metis not_None_eq option.collapse right split_comp.none)
   apply clarsimp
-  apply (case_tac "\<Gamma>b ! i")
-   apply (simp add: split_comp.none)
-  apply (drule spec, drule(1) mp)+
-  apply (auto intro: split_comp.intros)
+  apply (case_tac a)
+    apply clarsimp
+  using option.collapse
+    apply (fastforce dest: option.collapse simp add: split_comp.simps)+
   done
 
 lemma ttsplit_bang_inner_Cons:
@@ -510,7 +512,7 @@ next
 
 next
 
-  note split_if[split del]
+  note if_split[split del]
   case u_sem_if show ?case using u_sem_if.prems u_sem_if.hyps(1, 3)
     apply -
     apply (erule ttyping.cases, simp_all)
@@ -522,15 +524,15 @@ next
     apply (erule(1) u_tt_sem_pres_if)
      apply (rule u_sem_if.hyps(2), simp+)[1]
     apply (frule(2) preservation(1)[where \<tau>s=Nil, simplified, OF refl, OF _ _ _ u_sem_if.hyps(1)]
-     , erule ttyping_eq_typing[THEN iffD2, OF exI])
+        , erule ttyping_eq_typing[THEN iffD2, OF exI])
     apply (clarsimp simp: ttsplit_triv_def)
     apply (frule(2) frame_noalias_matches_ptrs)
     apply (frule(1) frame_noalias_matches_ptrs(2), blast)
-    apply (rule u_sem_if.hyps(4), simp split: split_if, assumption)
-     apply (simp split: split_if, erule(2) matches_ptrs_frame)
+    apply (rule u_sem_if.hyps(4), simp split: if_split, assumption)
+     apply (simp split: if_split, erule(2) matches_ptrs_frame)
      apply blast
     apply assumption
-    done 
+    done
 
 next
 
@@ -591,77 +593,138 @@ next
     done
 
 next
+  case (u_sem_take \<xi> \<gamma> \<sigma> x \<sigma>'' p r' fs f e)
 
-  case u_sem_take
-  have HELP2: "\<forall> \<tau>s. ((\<lambda>(a, b). type_repr a) \<circ> (\<lambda>(t, y). (instantiate \<tau>s t, y)))
-                   = (\<lambda>(t,y). type_repr (instantiate \<tau>s t))"
-  by (force split: prod.split)
-  show ?case using u_sem_take.prems u_sem_take.hyps(1, 3)
+  show ?case
+    using u_sem_take.prems(1)
+  proof (cases rule: ttyping.cases)
+    case (ttyping_take ijs t\<Gamma>3 t ts taken s t\<Gamma>4 k)
 
-    apply -
-    apply (erule ttyping.cases, simp_all)
-     apply (auto simp: composite_anormal_expr_def)[1]
-    apply (frule ttsplit_imp_split)
-    apply (frule matches_ptrs_noalias)
-    apply clarsimp
-    apply (frule(1) matches_ptrs_split', clarsimp)
-    apply (frule(2) preservation(1)[where \<tau>s=Nil, simplified, OF refl, OF _ _ _ u_sem_take.hyps(1)]
-     , erule ttyping_eq_typing[THEN iffD2, OF exI])
-    apply clarsimp
-    apply (erule u_t_p_recE, simp_all)
-    apply (erule u_tt_sem_pres_take)
-      apply (rule u_sem_take.hyps(2), simp+)[1]
-     apply assumption
-    apply (frule(2) frame_noalias_matches_ptrs)
-    apply (frule(1) frame_noalias_matches_ptrs(2), blast)
-    apply (frule(1) uval_typing_record_take, force, simp)
-    apply (elim conjE exE )
-    apply (frule(2) matches_ptrs_frame, blast)
-    apply (simp, erule disjE)
-     apply (clarsimp)
-     apply (frule(2) shareable_not_writable(1))
-     apply simp
-     (* FIXME: use new subgoal command or remove entirely.
-      * Note that legacy_subgoal pulls existing assumptions into "assms"
-      * and also leaves \<And>-quantified variables untouched.
-      * The proof below relies on both, and the new “subgoal” preserves neither. *)
-     legacy_subgoal
-       apply (rule u_sem_take.hyps(5) [simplified assms], simp+)
-        apply (case_tac taken)
-         apply (rule matches_ptrs_some [OF _ matches_ptrs_some])
-                 apply (simp)
-                using u_t_p_rec_w'
-                apply (force intro!: u_t_p_rec_w' simp: list_helper HELP2 map_update intro: list_helper [symmetric])
-               apply (simp)
-              apply (blast)
-             apply (blast)
-            apply (blast)
-           apply (blast)
-          apply (blast)
-         apply (blast)
-        apply (clarsimp)
-        apply (rule pointerset_helper_matches_ptrs)
-          apply (rule matches_ptrs_some [OF _ matches_ptrs_some])
-                  apply (simp)
-                 apply (force intro!: u_t_p_rec_w' simp: list_helper HELP2 map_update intro: list_helper [symmetric])
-                apply (simp)
-               apply (blast)
-              apply (blast)
-             apply (blast)
-            apply (blast)
-           apply (blast)
-          apply (blast)
-         apply (blast)
-        apply (blast)
-       apply (clarsimp)
-     done
-     legacy_subgoal
-       apply (rule u_sem_take.hyps(5) [simplified assms], simp+)
-       apply (rule matches_ptrs_some [OF _ matches_ptrs_some],assumption, erule(1) u_t_p_rec_w',simp)
-              apply (force simp add: map_update intro: list_helper[symmetric])
-             apply (simp+, blast+)
+    obtain \<Gamma>1 \<Gamma>2
+      where "[] \<turnstile> snd \<Gamma> \<leadsto> \<Gamma>1 | \<Gamma>2"
+        and snd_t\<Gamma>3_is: "snd t\<Gamma>3 = [] @ \<Gamma>1"
+        and snd_t\<Gamma>4_is: "snd t\<Gamma>4 = [Some t, Some (TRecord (ts[f := (t, taken)]) s)] @ \<Gamma>2"
+      using ttsplit_imp_split ttyping_take by blast
+    moreover then obtain r1 w1 r2 w2
+      where matches1: "\<Xi>, \<sigma> \<turnstile> \<gamma> matches \<Gamma>1 \<langle>r1, w1\<rangle>"
+        and matches2: "\<Xi>, \<sigma> \<turnstile> \<gamma> matches \<Gamma>2 \<langle>r2, w2\<rangle>"
+        and r_as_un: "r = r1 \<union> r2"
+        and w_as_un: "w = w1 \<union> w2"
+        and w1_w2_disjoint: "w1 \<inter> w2 = {}"
+      using matches_ptrs_split' u_sem_take.prems(3) by blast
+    moreover then have
+      w1_r2_noalias: "w1 \<inter> r2 = {}"
+      and w2_r1_noalias: "w2 \<inter> r1 = {}"
+      using matches_ptrs_noalias u_sem_take.prems(3) by blast+
+
+    have "\<Xi>, [], \<Gamma>1 \<turnstile> x : TRecord ts s"
+      using snd_t\<Gamma>3_is ttyping_imp_typing ttyping_take by fastforce
+    then obtain r1' w1'
+      where uptr_p_under_\<sigma>'': "\<Xi>, \<sigma>'' \<turnstile> UPtr p r' :u TRecord ts s \<langle>r1', w1'\<rangle>"
+        and r1'_sub: "r1' \<subseteq> r1"
+        and frame1: "frame \<sigma> w1 \<sigma>'' w1'"
+      using preservation(1)[where \<tau>s=Nil, simplified]
+        u_sem_take.prems(2,4) matches1 u_sem_take.hyps(1)
+      by blast
+
+    have matches2_under_\<sigma>'': "\<Xi>, \<sigma>'' \<turnstile> \<gamma> matches \<Gamma>2 \<langle>r2, w2\<rangle>"
+      using matches2 frame1 matches_ptrs_frame w1_w2_disjoint w1_r2_noalias
+      by blast
+
+    obtain w1'' fs'
+      where uptr_p_elim_lemmas:
+        "w1' = insert p w1''"
+        "\<Xi>, \<sigma>'' \<turnstile>* fs' :ur ts \<langle>r1', w1''\<rangle>"
+        "\<sigma>'' p = Some (URecord fs')"
+        "r' = RRecord (map (\<lambda>(a, b). type_repr a) ts)"
+        "s = Writable"
+        "p \<notin> w1''"
+        "p \<notin> r1'"
+      using uptr_p_under_\<sigma>''
+      by (auto simp add: ttyping_take)
+    then have t_wellformed: "[] \<turnstile> t wellformed"
+      using uval_typing_record_nth' ttyping_take
+      by auto
+    then obtain rf wf r1a w1a
+      where ut_fs_at_f: "\<Xi>, \<sigma>'' \<turnstile> fst (fs' ! f) :u t \<langle>rf, wf\<rangle>"
+        and ut_fs_taken_f: "\<Xi>, \<sigma>'' \<turnstile>* fs' :ur ts[f := (t, True)] \<langle>r1a, w1a\<rangle>"
+        and r1'_is: "r1' = rf \<union> r1a"
+        and w1''_is: "w1'' = wf \<union> w1a"
+        and "wf \<inter> w1a = {}"
+      using uval_typing_record_take uptr_p_elim_lemmas ttyping_take t_wellformed
+      by blast
+    then have uval_fs_f: "\<Xi>, \<sigma>'' \<turnstile> fst (fs ! f) :u t \<langle>rf, wf\<rangle>"
+      using u_sem_take.hyps uptr_p_elim_lemmas ut_fs_at_f by auto
+
+    have disjointness_lemmas:
+      "({p} \<union> wf \<union> w1a) \<inter> w2 = {}"
+      "({p} \<union> wf \<union> w1a) \<inter> r2 = {}"
+      "(rf \<union> r1a) \<inter> (wf \<union> w1a) = {}"
+      "{p} \<inter> (wf \<union> w1a) = {}"
+      "{p} \<inter> (rf \<union> r1a) = {}"
+      "wf \<inter> w1a = {}"
+      "w2 \<inter> (rf \<union> r1a) = {}"
+      using frame_noalias_matches_ptrs(1)[OF frame1 matches2 w1_w2_disjoint]
+        frame_noalias_matches_ptrs(2)[OF frame1 matches2 w1_r2_noalias]
+        r1'_is  w1''_is uptr_p_elim_lemmas
+            apply (force+)[2]
+      using uptr_p_elim_lemmas uval_typing_pointers_noalias(2) r1'_is  w1''_is
+          apply metis
+      using uptr_p_elim_lemmas u_t_p_rec_w w1''_is r1'_is
+         apply (blast+)[2]
+      using \<open>wf \<inter> w1a = {}\<close>
+       apply assumption
+      using r1'_is r1'_sub w2_r1_noalias
+      apply blast
       done
-    done
+
+    have "\<Xi>, \<xi>, fst (fs ! f) # UPtr p r' # \<gamma>, [], t\<Gamma>4, \<tau> T\<turnstile> (\<sigma>'', e) \<Down>! (\<sigma>', v)"
+    proof (cases taken)
+      case True
+
+      show ?thesis
+        using u_sem_take.prems ttyping_take
+      proof (intro u_sem_take.hyps(5))
+        show "\<Xi>, \<sigma>'' \<turnstile> fst (fs ! f) # UPtr p r' # \<gamma> matches snd t\<Gamma>4 \<langle>rf \<union> (r1a \<union> r2), wf \<union> (insert p w1a \<union> w2)\<rangle>"
+          using ut_fs_at_f matches2_under_\<sigma>'' disjointness_lemmas
+        proof (simp only: snd_t\<Gamma>4_is append_Cons append.left_neutral, intro matches_ptrs_some[OF _ matches_ptrs_some])
+          have "\<Xi>, \<sigma>'' \<turnstile>* fs :ur ts[f := (t, taken)] \<langle>r1a, w1a\<rangle>"
+            using True u_sem_take.hyps uptr_p_elim_lemmas ut_fs_taken_f by auto
+          moreover have "r' = RRecord (map (type_repr \<circ> fst) (ts[f := (t, taken)]))"
+            using uptr_p_elim_lemmas ttyping_take
+            by (simp add: case_prod_beta' list_helper map_update)
+          ultimately show "\<Xi>, \<sigma>'' \<turnstile> UPtr p r' :u TRecord (ts[f := (t, taken)]) s \<langle>r1a, insert p w1a\<rangle>"
+            using u_sem_take.hyps uptr_p_elim_lemmas uptr_p_under_\<sigma>'' ut_fs_taken_f r1'_is w1''_is
+            by (fastforce
+                simp add: uptr_p_elim_lemmas ttyping_take map_update
+                intro!: u_t_p_rec_w' distinct_list_update)
+        qed (force simp add: uval_fs_f)+
+      qed simp+
+    next
+      case False
+      then have wf_empty: "wf = {}"
+        using shareable_not_writable(1) ut_fs_at_f ttyping_take
+        by blast
+
+      show ?thesis
+        using u_sem_take.prems ttyping_take uval_fs_f
+      proof (intro u_sem_take.hyps(5))
+        show "\<Xi>, \<sigma>'' \<turnstile> fst (fs ! f) # UPtr p r' # \<gamma> matches snd t\<Gamma>4 \<langle>rf \<union> ((rf \<union> r1a) \<union> r2), {} \<union> (insert p w1a \<union> w2)\<rangle>"
+          using ut_fs_at_f matches2_under_\<sigma>'' disjointness_lemmas wf_empty
+        proof (simp only: snd_t\<Gamma>4_is append_Cons append.left_neutral, intro matches_ptrs_some[OF _ matches_ptrs_some])
+          have "ts[f := (t, False)] = ts"
+            by (simp add: list_helper ttyping_take)
+          thus "\<Xi>, \<sigma>'' \<turnstile> UPtr p r' :u TRecord (ts[f := (t, taken)]) s \<langle>rf \<union> r1a, insert p w1a\<rangle>"
+            using uptr_p_elim_lemmas wf_empty r1'_is uptr_p_under_\<sigma>'' w1''_is False by auto
+        qed (force simp add: uval_fs_f[simplified wf_empty])+
+      qed simp+
+    qed
+    moreover have "\<Xi>, \<xi>, \<gamma>, [], t\<Gamma>3, TRecord ts s T\<turnstile> (\<sigma>, x) \<Down>! (\<sigma>'', UPtr p r')"
+      using u_sem_take.hyps(2) u_sem_take.prems ttyping_take matches1 snd_t\<Gamma>3_is by auto
+    ultimately show "\<Xi>, \<xi>, \<gamma>, [], \<Gamma>, \<tau> T\<turnstile> (\<sigma>, Take x f e) \<Down>! (\<sigma>', v)"
+      using ttyping_take u_sem_take.hyps uptr_p_elim_lemmas
+      by (slowsimp intro!: u_tt_sem_pres_take)
+  qed (simp add: composite_anormal_expr_def)
 next
 
   case u_sem_take_ub show ?case using u_sem_take_ub.prems u_sem_take_ub.hyps(1, 3)
@@ -741,11 +804,10 @@ next
      apply (auto dest: ttyping_imp_typing)
     done
 
-qed  (fastforce intro!: u_tt_sem_pres_default
-               intro: u_sem_u_sem_all.intros
-               simp: composite_anormal_expr_def
-               dest: ttyping_imp_typing
-               )+
+qed  (auto intro!: u_tt_sem_pres_default
+           intro: u_sem_u_sem_all.intros
+           simp: composite_anormal_expr_def
+           dest: ttyping_imp_typing)+
 
 lemma u_tt_sem_pres_imp_u_sem:
   "\<Xi>, \<xi>, \<gamma>, [], \<Gamma>, \<tau> T\<turnstile> (\<sigma>, x) \<Down>! (\<sigma>', uv)
